coq/ApplyTySm.v
@@ -1,0 +1,209 @@
+Require Import LibTactics.
+Require Import Coq.micromega.Lia.
+Require Import LN_Lemmas.
+Require Export DistSubtyping.
+Require Import ApplyTy.
+
+(************************ Notations related to types **************************)
+Notation "[ z ~~> u ] t" := (typsubst_typ u z t) (at level 0).
+Notation "t ^-^ u"       := (open_typ_wrt_typ t u) (at level 67).
+Notation "t -^ x"        := (open_typ_wrt_typ t (t_tvar_f x))(at level 67).
+Notation "[[ A ]]"       := (typefv_typ A) (at level 0).
+Notation "A <: B"        := (declarative_subtyping A B)
+                              (at level 65, B at next level, no associativity) : type_scope.
+
+
+(***** Properties of local closure *****)
+
+Lemma napplytysm_lc_1 : forall A B, NApplyTySimple A B -> lc_typ A.
+Proof.  introv H.  induction* H.  Qed.
+
+Lemma napplytysm_lc_2 : forall A B, NApplyTySimple A B -> lc_Fty B.
+Proof.  introv H.  induction* H.  Qed.
+
+#[export] Hint Immediate napplytysm_lc_1 napplytysm_lc_2 : core.
+
+
+Lemma applytysm_lc_1 : forall A B C, ApplyTySimple A B C -> lc_typ A.
+Proof.  introv H.  induction* H.  Qed.
+
+Lemma applytysm_lc_2 : forall A B C, ApplyTySimple A B C -> lc_Fty B.
+Proof.  introv H.  induction* H. Qed.
+
+Lemma applytysm_lc_3 : forall A B C, ApplyTySimple A B C -> lc_typ C.
+Proof.  introv H.  induction~ H. inverts H. eauto with lngen. Qed.
+
+#[export] Hint Immediate applytysm_lc_1 applytysm_lc_2 applytysm_lc_3 : core.
+
+
+(************************ Proofs **************************)
+(* ApplyTySimple and ApplyTy are exactly the same when the argument type is union
+   ordinary. *)
+Lemma applyTySimple_applyTy : forall A BFty,
+    UnionOrdinaryFty BFty ->
+    (forall C, (ApplyTySimple A BFty C <-> ApplyTy A BFty C) /\
+                 (NApplyTySimple A BFty <-> NApplyTy A BFty)).
+Proof.
+  intro A.
+  induction A; intros BFTy Hord; repeat split; intro Happ.
+  (* Every case is dealt with either by finding a contradiction with the ordu
+     constraint, or through a straightforward application of the induction
+     hypotheses. *)
+  Local Ltac solve_with_IH H Hord IHA1 IHA2 :=
+    inverts H;
+    now first
+      [
+        inverts Hord; exfalso; now find_contradiction_on_split
+      | constructor; auto; solve [ apply IHA1; auto | apply IHA2; auto ]
+      ].
+  all: solve [solve_with_IH Happ Hord IHA1 IHA2].
+Qed.
+
+Lemma splu_ind AFty P :
+    (forall AFty, UnionOrdinaryFty AFty -> P AFty) ->
+    (forall A A1 A2, splu A A1 A2 ->
+                     P A1 ->
+                     P A2
+                     -> P (fty_StackArg A)) ->
+    P AFty.
+Proof.
+(* TODO *)
+Admitted.
+
+Lemma applyTySimple_excl_mid : forall A B,
+    (exists C, ApplyTySimple A B C) \/
+      (NApplyTySimple A B).
+Proof.
+  (* TODO *)
+Admitted.
+
+Lemma applyTySimple_inter_l : forall A1 A2 B C,
+  ApplyTySimple A1 (fty_StackArg B) C ->
+  exists C', ApplyTySimple (A1 & A2) (fty_StackArg B) C' /\ C' <: C.
+Proof.
+  intros A1 A2 B C1 Happ.
+  forwards H: applyTySimple_excl_mid A2 (fty_StackArg B).
+  destruct H as [ [C2 ?] | ]; eexists; eauto.
+Qed.
+
+Lemma applyTySimple_inter_r : forall A1 A2 B C,
+  ApplyTySimple A2 (fty_StackArg B) C ->
+  exists C', ApplyTySimple (A1 & A2) (fty_StackArg B) C' /\ C' <: C.
+Proof.
+  intros A1 A2 B C2 Happ.
+  forwards H: applyTySimple_excl_mid A1 (fty_StackArg B).
+  destruct H as [ [C1 ?] | ]; eexists; eauto.
+Qed.
+
+Lemma mono_applyTySimple_argu : forall A B C B',
+        ApplyTySimple A (fty_StackArg B) C ->
+        B' <: B ->
+        exists C',
+          ApplyTySimple A (fty_StackArg B') C' /\
+          C' <: C.
+Proof.
+  intros A.
+  induction A;
+  introv H; try solve [inverts H].
+  - intros.
+    inverts H;
+      try (specializes IHA1;
+          [ eassumption | eassumption | destruct IHA1 as [C1' [? ? ]  ] ]);
+      try (specializes IHA2;
+          [ eassumption | eassumption | destruct IHA2 as [C2' [? ? ]  ] ]).
+    + forwards Hinter: applyTySimple_inter_l; [ eassumption | ].
+      destruct Hinter as [ C' [? ?] ].
+      eauto.
+    + forwards Hinter: applyTySimple_inter_r; [ eassumption | ].
+      destruct Hinter as [ C' [? ?] ].
+      eauto.
+    + do 2 eexists; eauto.
+  - intros. inverts H.
+    specializes IHA1;
+          [eassumption | eassumption | destruct IHA1 as [C1' [? ?] ] ].
+    specializes IHA2;
+          [eassumption | eassumption | destruct IHA2 as [C2' [? ?] ] ].
+    do 2 eexists.
+    + eauto.
+    + convert2asub; solve_algo_sub; eauto.
+  - intros. inverts H.
+    eexists.
+    eauto.
+  - intros. inverts H.
+    exists t_bot.
+    eauto. splits; auto.
+Qed.
+
+Lemma inv_applyTySimple_argu : forall A B C B1 B2 ,
+        ApplyTySimple A (fty_StackArg B) C ->
+        splu B B1 B2 ->
+        exists C1 C2,
+          ApplyTySimple A (fty_StackArg B1) C1 /\
+          ApplyTySimple A (fty_StackArg B2) C2 /\
+          C1 <: C /\
+          C2 <: C.
+Proof.
+  introv Happ Hspl.
+  lets H: dsub_splu Hspl.
+  destruct H as [? ?].
+  forwards H1: mono_applyTySimple_argu A B C B1; eauto.
+  forwards H2: mono_applyTySimple_argu A B C B2; eauto.
+  destruct H1 as [C1' [? ?] ].
+  destruct H2 as [C2' [? ?] ].
+  do 2 eexists.
+  eauto.
+Qed.
+
+
+Lemma applyTySimple_approx : forall A BFty C,
+    ApplyTySimple A BFty C ->
+    exists C', ApplyTy A BFty C' /\
+             C' <: C.
+Proof.
+  intros A ?.
+  applys splu_ind BFty; clear BFty.
+  - intros BFty Hord C.
+    intros.
+    exists C.
+    forwards Hiff: applyTySimple_applyTy; [eassumption | ].
+    destruct Hiff as [Hiff _].
+    split; [apply Hiff | ]; eauto.
+  - intros B B1 B2 Hspl IHB1 IHB2 C Happ.
+    forwards H: inv_applyTySimple_argu; try eassumption.
+    destruct H as [C1 [C2 [HB1 [HB2 [? ?] ] ] ] ].
+    specializes IHB1; eauto.
+    destruct IHB1 as [C1' [? ? ] ].
+    specializes IHB2; eauto.
+    destruct IHB2 as [C2' [? ?] ].
+    eexists. split.
+    eapply ApplyTyUnionArg; eauto.
+    convert2asub.
+    solve_algo_sub;
+    eauto using algo_trans.
+Qed.
+
+Lemma applyTySimple_subst : forall A B C U X,
+    ApplyTySimple A (fty_StackArg B) C ->
+    lc_typ U ->
+    exists C', ApplyTySimple ([X ~~> U] A) ([X ~~> U] B) C' /\
+           C' <: [X ~~> U] C.
+Proof.
+  intros A B C U X.
+  intros Happ ?.
+  induction A; cbn; eexists; inverts Happ; cbn.
+  - admit. (* TODO hard cases *)
+  - admit.
+  - admit.
+  - admit.
+
+  - splits.
+    constructor.
+    + admit. (* TODO lc *)
+    + convert2asub.
+      apply typsubst_typ_algo_sub; auto.
+    + constructor.
+      admit. (* TODO lc *)
+  - splits; auto.
+    constructor.
+    admit. (* TODO loc *)
+Qed.
